compose/SimSystem.v
@@ -1,0 +1,19 @@
+Require Import EventsC.
+Require Import Values.
+Require Import AST.
+Require Import Memory.
+Require Import Globalenvs.
+Require Import Smallstep Simulation.
+Require Import CoqlibC.
+
+Require Import Mod ModSem Skeleton System.
+Require Import SimMem Sound SimSymb.
+
+Set Implicit Arguments.
+
+
+Section SIM.
+  Context `{SM: SimMem.class}.
+  Context `{SU: Sound.class}.
+  Context {SS: SimSymb.class SM}.
+End SIM.
