proof/Sound.v
@@ -113,9 +113,10 @@ Module Sound.
         (INCL: SkEnv.includes skenv_link sk),
         <<SKE: su.(skenv) m0 skenv0>>;
 
-    system_skenv: forall su m0 skenv_link
+    system_skenv: forall su m0 sk_link skenv_link
+        (LOAD: Sk.load_skenv sk_link = skenv_link)
         (SKELINK: su.(skenv) m0 skenv_link),
-        <<SKE: su.(skenv) m0 (System.skenv skenv_link)>>;
+         <<SKESYS: su.(skenv) m0 (System.skenv sk_link skenv_link)>>;
 
     system_axiom: forall
         ef skenv0 su0 args0
